arch_split: change caps_of_state to be explicit projection f caps_of_state

proof/invariant-abstract/CSpaceInv_AI.thy
@@ -13,15 +13,26 @@ CSpace invariants
 *)
 
 theory CSpaceInv_AI
-imports ArchAcc_AI
+imports "./$L4V_ARCH/ArchCSpaceInv_AI"
 begin
+
+unqualify_consts (in Arch)
+  cap_master_arch_cap :: "arch_cap \<Rightarrow> arch_cap"
+  table_cap_ref :: "arch_cap \<Rightarrow> vs_ref list option"
+      
+unqualify_facts (in Arch)
+  valid_validate_vm_rights[simp]
+  aobj_ref_acap_rights_update[simp]
+  arch_obj_size_acap_rights_update[simp]
+  valid_arch_cap_acap_rights_update[intro]
+  cap_master_arch_inv[simp]
 
 lemma remove_rights_cap_valid[simp]:
   "s \<turnstile> c \<Longrightarrow> s \<turnstile> remove_rights S c"
-  using valid_validate_vm_rights[simplified valid_vm_rights_def]
-  by (cases c, simp_all add: remove_rights_def cap_rights_update_def
-                   valid_cap_def cap_aligned_def acap_rights_update_def
-                 split: arch_cap.splits)
+  using valid_validate_vm_rights
+  apply (cases c, simp_all add: remove_rights_def cap_rights_update_def
+                   valid_cap_def cap_aligned_def)
+  by fastforce
 
 
 lemma get_thread_state_inv [simp]:
@@ -242,68 +253,7 @@ lemma valid_reply_masters_tcb_update:
                      cte_wp_at_after_update obj_at_def)
 
 
-lemma valid_arch_obj_tcb_update':
-  "\<lbrakk> valid_arch_obj obj s; kheap s p = Some (TCB t) \<rbrakk>
-   \<Longrightarrow> valid_arch_obj obj (s\<lparr>kheap := kheap s(p \<mapsto> TCB t')\<rparr>)"
-  apply (cases obj)
-     apply (fastforce elim: typ_at_same_type [rotated -1])
-    apply clarsimp
-    apply (rename_tac "fun" x)
-    apply (erule_tac x=x in allE)
-    apply (case_tac "fun x", (clarsimp simp: obj_at_def)+)[1]
-   apply clarsimp
-   apply (rename_tac "fun" x)
-   apply (erule_tac x=x in ballE)
-   apply (case_tac "fun x", (clarsimp simp: obj_at_def)+)[1]
-   apply (fastforce elim: typ_at_same_type [rotated -1])
-  apply simp
-  done
 
-
-lemma valid_arch_obj_tcb_update:
-  "kheap s p = Some (TCB t)
-   \<Longrightarrow> valid_arch_obj obj (s\<lparr>kheap := kheap s(p \<mapsto> TCB t')\<rparr>) = valid_arch_obj obj s"
-  apply (rule iffI)
-   apply (drule valid_arch_obj_tcb_update'[where p=p and t'=t], simp)
-   apply (simp add: fun_upd_idem)
-  apply (erule(1) valid_arch_obj_tcb_update')
-  done
-
-
-lemma valid_arch_objs_tcb_update:
-  "\<lbrakk> valid_arch_objs s; kheap s p = Some (TCB t)\<rbrakk>
-    \<Longrightarrow> valid_arch_objs (s\<lparr>kheap := kheap s(p \<mapsto> TCB t')\<rparr>)"
-  apply (erule valid_arch_objs_stateI)
-    apply (clarsimp simp: obj_at_def vs_refs_def split: split_if_asm)
-   apply simp
-  apply (clarsimp simp: obj_at_def valid_arch_obj_tcb_update split: split_if_asm)
-  done
-
-
-lemma vs_lookup1_tcb_update:
-  "kheap s p = Some (TCB t)
-      \<Longrightarrow> vs_lookup1 (s\<lparr>kheap := kheap s(p \<mapsto> TCB t')\<rparr>) = vs_lookup1 s"
-  by (clarsimp simp add: vs_lookup1_def obj_at_def vs_refs_def intro!: set_eqI)
-
-
-lemma vs_lookup_tcb_update:
-  "kheap s p = Some (TCB t)
-      \<Longrightarrow> vs_lookup (s\<lparr>kheap := kheap s(p \<mapsto> TCB t')\<rparr>) = vs_lookup s"
-  by (clarsimp simp add: vs_lookup_def vs_lookup1_tcb_update)
-
-
-lemma only_idle_tcb_update:
-  "\<lbrakk>only_idle s; ko_at (TCB t) p s; tcb_state t = tcb_state t' \<or> \<not>idle (tcb_state t') \<rbrakk>
-    \<Longrightarrow> only_idle (s\<lparr>kheap := kheap s(p \<mapsto> TCB t')\<rparr>)"
-  by (clarsimp simp: only_idle_def pred_tcb_at_def obj_at_def)
-
-
-lemma tcb_update_global_pd_mappings:
-  "\<lbrakk> valid_global_pd_mappings s; ko_at (TCB t) p s \<rbrakk>
-       \<Longrightarrow> valid_global_pd_mappings (s\<lparr>kheap := kheap s(p \<mapsto> TCB t')\<rparr>)"
-  apply (erule valid_global_pd_mappings_pres)
-     apply (clarsimp simp: obj_at_def)+
-  done
 
 
 lemma tcb_state_same_cte_wp_at:
@@ -395,16 +345,7 @@ where
  | cap.DomainCap \<Rightarrow> cap.DomainCap
  | cap.ReplyCap ref master \<Rightarrow> cap.ReplyCap ref True
  | cap.UntypedCap ref n f \<Rightarrow> cap.UntypedCap ref n 0
- | cap.ArchObjectCap acap \<Rightarrow> cap.ArchObjectCap (case acap of
-      arch_cap.PageCap ref rghts sz mapdata \<Rightarrow>
-         arch_cap.PageCap ref UNIV sz None
-    | arch_cap.ASIDPoolCap pool asid \<Rightarrow>
-         arch_cap.ASIDPoolCap pool 0
-    | arch_cap.PageTableCap ptr data \<Rightarrow>
-         arch_cap.PageTableCap ptr None
-    | arch_cap.PageDirectoryCap ptr data \<Rightarrow>
-         arch_cap.PageDirectoryCap ptr None
-       | _ \<Rightarrow> acap)
+ | cap.ArchObjectCap acap \<Rightarrow> cap.ArchObjectCap (cap_master_arch_cap acap)
  | _ \<Rightarrow> cap"
 
 
@@ -434,19 +375,10 @@ lemma cap_master_cap_eqDs1:
   "cap_master_cap cap = cap.ReplyCap ref master
      \<Longrightarrow> master = True
           \<and> (\<exists>master. cap = cap.ReplyCap ref master)"
-  "cap_master_cap cap = cap.ArchObjectCap (arch_cap.PageCap ref rghts sz mapdata)
-     \<Longrightarrow> rghts = UNIV \<and> mapdata = None
-          \<and> (\<exists>rghts mapdata. cap = cap.ArchObjectCap (arch_cap.PageCap ref rghts sz mapdata))"
-  "cap_master_cap cap = cap.ArchObjectCap arch_cap.ASIDControlCap
-     \<Longrightarrow> cap = cap.ArchObjectCap arch_cap.ASIDControlCap"
-  "cap_master_cap cap = cap.ArchObjectCap (arch_cap.ASIDPoolCap pool asid)
-     \<Longrightarrow> asid = 0 \<and> (\<exists>asid. cap = cap.ArchObjectCap (arch_cap.ASIDPoolCap pool asid))"
-  "cap_master_cap cap = cap.ArchObjectCap (arch_cap.PageTableCap ptr data)
-     \<Longrightarrow> data = None \<and> (\<exists>data. cap = cap.ArchObjectCap (arch_cap.PageTableCap ptr data))"
-  "cap_master_cap cap = cap.ArchObjectCap (arch_cap.PageDirectoryCap ptr data2)
-     \<Longrightarrow> data2 = None \<and> (\<exists>data2. cap = cap.ArchObjectCap (arch_cap.PageDirectoryCap ptr data2))"
+  "cap_master_cap cap = ArchObjectCap acap
+     \<Longrightarrow> \<exists>ac. cap = ArchObjectCap ac \<and> acap = cap_master_arch_cap ac"
   by (clarsimp simp: cap_master_cap_def
-              split: cap.split_asm arch_cap.split_asm)+
+              split: cap.split_asm)+
 
 
 lemmas cap_master_cap_eqDs = cap_master_cap_eqDs1 cap_master_cap_eqDs1 [OF sym]
@@ -476,13 +408,7 @@ lemma cap_badge_simps [simp]:
  "cap_badge (cap.ArchObjectCap cap)                = None"
   by (auto simp: cap_badge_def)
 
-(* FIXME: move to somewhere sensible *)
-lemma pageBitsForSize_simps[simp]:
-  "pageBitsForSize ARMSmallPage    = 12"
-  "pageBitsForSize ARMLargePage    = 16"
-  "pageBitsForSize ARMSection      = 20"
-  "pageBitsForSize ARMSuperSection = 24"
-  by (simp add: pageBitsForSize_def)+
+
 
 
 lemma cdt_parent_of_def:
@@ -842,8 +768,8 @@ crunch it[wp]: set_cap "\<lambda>s. P (idle_thread s)"
 
 lemma set_cap_refs [wp]:
   "\<lbrace>\<lambda>x. P (global_refs x)\<rbrace> set_cap cap p \<lbrace>\<lambda>_ x. P (global_refs x)\<rbrace>"
-  apply (simp add: global_refs_def)
-  apply wpx
+  apply (rule global_refs_lift)
+  apply wp
   done
 
 
@@ -1202,38 +1128,70 @@ lemma get_cap_caps_of_state:
   "(fst (get_cap p s) = {(cap, s)}) = (Some cap = caps_of_state s p)"
   by (clarsimp simp: caps_of_state_def eq_commute)
 
+definition
+  "arch_cap_fun_lift P F c \<equiv> case c of ArchObjectCap ac \<Rightarrow> P ac | _ \<Rightarrow> F"
 
+lemmas arch_cap_fun_lift_simps[simp] =
+  arch_cap_fun_lift_def[split_simps cap.split]
+
+definition "table_cap_ref_gen c \<equiv> arch_cap_fun_lift table_cap_ref None c"
+
+lemmas table_cap_ref_gen_simps[simp] =
+  table_cap_ref_gen_def[simplified arch_cap_fun_lift_def, split_simps cap.split]
+                                                            
 definition
   no_cap_to_obj_with_diff_ref :: "cap \<Rightarrow> cslot_ptr set \<Rightarrow> 'z::state_ext state \<Rightarrow> bool"
 where
  "no_cap_to_obj_with_diff_ref cap S \<equiv>
   \<lambda>s. \<forall>p \<in> UNIV - S. \<not> cte_wp_at (\<lambda>c. obj_refs c = obj_refs cap \<and>
-                                       \<not> (table_cap_ref c = table_cap_ref cap)) p s"
+                                     \<not> (table_cap_ref_gen c = table_cap_ref_gen cap)
+                                      ) p s"
 
+context Arch begin
+ 
+lemma abj_ref_none_no_refs:
+  "aobj_ref ac = None \<Longrightarrow> table_cap_ref ac = None"
+  unfolding table_cap_ref_def
+  by (cases ac; simp)
 
-lemma obj_ref_none_no_asid:
-  "{} = obj_refs new_cap \<longrightarrow> None = table_cap_ref new_cap"
-  "obj_refs new_cap = {} \<longrightarrow> table_cap_ref new_cap = None"
-  by (simp add: table_cap_ref_def split: cap.split arch_cap.split)+
+unqualify_facts 
+  abj_ref_none_no_refs
 
+end
 
 lemma no_cap_to_obj_with_diff_ref_Null:
   "no_cap_to_obj_with_diff_ref cap.NullCap S = \<top>"
-  by (rule ext, simp add: no_cap_to_obj_with_diff_ref_def
-                          cte_wp_at_caps_of_state obj_ref_none_no_asid)
+  apply (rule ext, clarsimp simp add: no_cap_to_obj_with_diff_ref_def
+                          cte_wp_at_caps_of_state)
+  by (rule cap_cases; fastforce intro: abj_ref_none_no_refs)
 
 
-definition
-  "is_ap_cap cap \<equiv> case cap of cap.ArchObjectCap (arch_cap.ASIDPoolCap ap asid) \<Rightarrow> True | _ \<Rightarrow> False"
+context Arch begin
+  unqualify_consts reachable_pg_cap
+(*
 
+  \<and> (\<forall>vref. vs_cap_ref cap = Some vref
+                \<longrightarrow> (vs_cap_ref newcap = Some vref
+                       \<and> obj_refs newcap = obj_refs cap)
+                 \<or> (\<forall>oref \<in> obj_refs cap. \<not> (vref \<unrhd> oref) s))
+      \<and> no_cap_to_obj_with_diff_ref newcap {sl} s
+      \<and> ((is_pt_cap newcap \<or> is_pd_cap newcap) \<longrightarrow> cap_asid newcap = None
+          \<longrightarrow> (\<forall>r \<in> obj_refs newcap. obj_at (empty_table (set (arm_global_pts (arch_state s)))) r s))
+      \<and> ((is_pt_cap newcap \<or> is_pd_cap newcap)
+             \<longrightarrow> ((is_pt_cap newcap \<and> is_pt_cap cap \<or> is_pd_cap newcap \<and> is_pd_cap cap)
+                      \<longrightarrow> (cap_asid newcap = None \<longrightarrow> cap_asid cap = None)
+                      \<longrightarrow> obj_refs cap \<noteq> obj_refs newcap)
+             \<longrightarrow> (\<forall>sl'. cte_wp_at (\<lambda>cap'. obj_refs cap' = obj_refs newcap
+                                           \<and> (is_pd_cap newcap \<and> is_pd_cap cap' \<or> is_pt_cap newcap \<and> is_pt_cap cap')
+                                           \<and> (cap_asid newcap = None \<or> cap_asid cap' = None)) sl' s \<longrightarrow> sl' = sl))
+      \<and> \<not>is_ap_cap newcap)
 
-lemmas is_ap_cap_simps [simp] = is_ap_cap_def [split_simps cap.split arch_cap.split]
+*)
+end
 
-
-definition
-  "reachable_pg_cap cap \<equiv> \<lambda>s.
-   is_pg_cap cap \<and>
-   (\<exists>vref. vs_cap_ref cap = Some vref \<and> (vref \<unrhd> obj_ref_of cap) s)"
+abbreviation
+  reachable_pg_cap_gen where
+  "reachable_pg_cap_gen \<equiv> arch_cap_fun_lift reachable_pg_cap \<bottom>"
 
 
 definition
@@ -1241,7 +1199,7 @@ definition
 where
  "replaceable s sl newcap \<equiv> \<lambda>cap.
     (cap = newcap)
-  \<or> (\<not> is_final_cap' cap s \<and> newcap = cap.NullCap \<and> \<not> reachable_pg_cap cap s)
+  \<or> (\<not> is_final_cap' cap s \<and> newcap = cap.NullCap \<and> \<not> reachable_pg_cap_gen cap s)
   \<or> (is_final_cap' cap s
       \<and> (\<forall>p\<in>zobj_refs cap - zobj_refs newcap.
               obj_at (Not \<circ> live) p s)
@@ -1261,22 +1219,8 @@ where
       \<and> \<not> is_untyped_cap newcap \<and> \<not> is_master_reply_cap newcap
       \<and> \<not> is_reply_cap newcap
       \<and> newcap \<noteq> cap.IRQControlCap
-      \<and> (newcap \<noteq> cap.NullCap \<longrightarrow> cap_class newcap = cap_class cap)
-      \<and> (\<forall>vref. vs_cap_ref cap = Some vref
-                \<longrightarrow> (vs_cap_ref newcap = Some vref
-                       \<and> obj_refs newcap = obj_refs cap)
-                 \<or> (\<forall>oref \<in> obj_refs cap. \<not> (vref \<unrhd> oref) s))
-      \<and> no_cap_to_obj_with_diff_ref newcap {sl} s
-      \<and> ((is_pt_cap newcap \<or> is_pd_cap newcap) \<longrightarrow> cap_asid newcap = None
-          \<longrightarrow> (\<forall>r \<in> obj_refs newcap. obj_at (empty_table (set (arm_global_pts (arch_state s)))) r s))
-      \<and> ((is_pt_cap newcap \<or> is_pd_cap newcap)
-             \<longrightarrow> ((is_pt_cap newcap \<and> is_pt_cap cap \<or> is_pd_cap newcap \<and> is_pd_cap cap)
-                      \<longrightarrow> (cap_asid newcap = None \<longrightarrow> cap_asid cap = None)
-                      \<longrightarrow> obj_refs cap \<noteq> obj_refs newcap)
-             \<longrightarrow> (\<forall>sl'. cte_wp_at (\<lambda>cap'. obj_refs cap' = obj_refs newcap
-                                           \<and> (is_pd_cap newcap \<and> is_pd_cap cap' \<or> is_pt_cap newcap \<and> is_pt_cap cap')
-                                           \<and> (cap_asid newcap = None \<or> cap_asid cap' = None)) sl' s \<longrightarrow> sl' = sl))
-      \<and> \<not>is_ap_cap newcap)"
+      \<and> (newcap \<noteq> cap.NullCap \<longrightarrow> cap_class newcap = cap_class cap))
+      "
 
 
 lemma range_not_empty_is_physical:
